

MATH 345 Homework 5 Solutions

Question 1

In SL-form:

$$-\frac{d}{dx}[(1+x^2)\phi'(x)] = \lambda\phi(x)$$

and we have $\phi(0) = 0$ and $\phi(1) = 0$

The Rayleigh quotient for a given u is:

$$R[u] = \frac{\int_0^1 p(x)[u'(x)]^2 dx}{\int_0^1 [u(x)]^2 dx} = \frac{\int_0^1 (1+x^2)[u'(x)]^2 dx}{\int_0^1 u(x)^2 dx}$$

for such u that satisfies the boundary conditions, we have $\lambda_1 \leq R[u]$

For our test function $u_T(x)$, the first eigenfunction should be positive on $(0, 1)$, satisfy $\phi(0) = 0, \phi(1) = 0$ and have 0 derivative at $x = 0$

since $u_T(0) = 0, u'_T(0) = 1 - 0 = 1, u_T(1) = 0$

$$u_T(x) = x(1-x)$$

$$[u_T(x)]^2 = [x(1-x)]^2 = x^2(1-x)^2 = x^2(1-2x+x^2) = x^2 - 2x^3 + x^4$$

$$u'_T(x) = x \cdot -1 + (1-x) \cdot 1 = 1 - 2x$$

$$[u'_T(x)]^2 = [1 - 2x]^2 = 1 - 2x - 2x + 4x^2 = 1 - 4x + 4x^2$$

Numerator:

$$\begin{aligned} N &= \int_0^1 (1+x^2)[u'_T(x)]^2 dx = \int_0^1 (1+x^2)(1-4x+4x^2) dx \\ &= \int_0^1 1 - 4x + 4x^2 + x^2 - 4x^3 + 4x^4 dx = \int_0^1 1 - 4x + 5x^2 - 4x^3 + 4x^4 dx \\ &= \left[x - 2x^2 + \frac{5}{3}x^3 - x^4 + \frac{4}{5}x^5 \right]_0^1 \\ &= 1 - 2 + \frac{5}{3} - 1 + \frac{4}{5} = \frac{7}{15} \end{aligned}$$

Denominator:

$$\begin{aligned} D &= \int_0^1 u_T(x)^2 dx = \int_0^1 x^2 - 2x^3 + x^4 dx \\ &= \left[\frac{1}{3}x^3 - \frac{1}{2}x^4 + \frac{1}{5}x^5 \right]_0^1 = \frac{1}{3} - \frac{1}{2} + \frac{1}{5} = \frac{1}{30} \end{aligned}$$

Our Rayleigh Q:

$$R[u_T] = \frac{N}{D} = \frac{7/15}{1/30} = 14$$

So reasonable upper bound for the smallest eigenvalue is $\boxed{\lambda_1 \leq 14}$ If we use higher order terms in our u_T function we can get more accurate estimates

Question 2

We have:

$$\frac{d}{dx} \left(p(x) \frac{d\phi}{dx} \right) + [\lambda \sigma(x) + q(x)] \phi = 0$$

with BCs $\frac{d\phi}{dx}(0) = 0$ and $\frac{d\phi}{dx}(L) = 0$

for $\lambda \gg 1$, $\lambda \sigma(x)$ dominates so we can drop $q(x)$. and we now have $(p\phi')' + \lambda \sigma \phi \approx 0$

$$\begin{aligned} \frac{\phi'' p}{p} + \frac{p' \phi}{p} + \frac{\lambda \sigma \phi}{p} &\approx 0 \\ \phi'' + \frac{p' \phi}{p} + \frac{\lambda \sigma \phi}{p} &\approx 0 \end{aligned}$$

using ansatz:

$$\phi(x) = A(x) \cos \theta(x)$$

$$\phi' = A' \cos \theta(x) - A \theta' \sin \theta(x)$$

$$\phi'' = (A'' - A(\theta')^2) \cos \theta - (2A' \theta' + A \theta'') \sin \theta$$

$$(A'' - A(\theta')^2) \cos \theta - (2A' \theta' + A \theta'') \sin \theta + \frac{\lambda \sigma}{p} A \cos \theta \approx 0$$

cos coefficient:

$$A \left(-(\theta')^2 + \lambda \frac{\sigma}{p} \right) + A''.$$

sin coefficient:

$$-(2A' \theta' + A \theta'')$$

For large λ , the terms $A(\theta')^2$ and $\lambda \frac{\sigma}{p} A$ are $O(\lambda)$, while A'' is $O(1)$; thus we can drop A'' at leading order:

$$-(\theta')^2 + \lambda \frac{\sigma(x)}{p(x)} \approx 0 \quad \Rightarrow \quad (\theta')^2 \approx \lambda \frac{\sigma(x)}{p(x)}$$

$$\theta'(x) \approx \sqrt{\lambda} \sqrt{\frac{\sigma(x)}{p(x)}}.$$

$$\theta(x) \approx \sqrt{\lambda} \int_0^x \sqrt{\frac{\sigma(s)}{p(s)}} ds + C$$

$$\phi(x) \approx A(x) \cos \left(\sqrt{\lambda} \int_0^x \sqrt{\frac{\sigma}{p}} ds + C \right)$$

using the Neumann boundary conditions

we have $\phi'(0) = \phi'(L) = 0$

$$\phi'(x) \approx -A \theta'(x) \sin \theta(x)$$

so

at $x = 0$:

$$\phi'(0) \approx -A\theta'(0) \sin \theta(0) = 0 \quad \Rightarrow \quad \sin \theta(0) \approx 0.$$

we can take $\theta(0) = 0$ (so $\delta = 0$)
at $x = L$:

$$\phi'(L) \approx -A\theta'(L) \sin \theta(L) = 0 \quad \Rightarrow \quad \sin \theta(L) \approx 0 \quad \Rightarrow \quad \theta(L) \approx n\pi, \quad n = 0, 1, 2, \dots$$

but

$$\theta(L) \approx \sqrt{\lambda} \int_0^L \sqrt{\frac{\sigma(s)}{p(s)}} ds = \sqrt{\lambda} J.$$

so the quantization condition is:

$$\sqrt{\lambda_n} J \approx n\pi \quad \Rightarrow \quad \boxed{\lambda_n \approx \frac{n^2 \pi^2}{J^2}}, \quad J = \int_0^L \sqrt{\frac{\sigma(x)}{p(x)}} dx$$

and the corresponding eigenfunctions (to leading order) are

$$\boxed{\phi_n(x) \approx A \cos \left(\frac{n\pi}{J} \int_0^x \sqrt{\frac{\sigma(s)}{p(s)}} ds \right)}$$

Question 3

WWS, for continuous $f : [0, \pi] \rightarrow \mathbb{R}$ (or even \mathbb{C}),

$$\sum_{k=1}^n \left| \int_0^\pi f(x) \sin(kx) dx \right|^2 \leq \frac{\pi}{2} \int_0^\pi |f(x)|^2 dx$$

using orthogonality of the sin
the inner product:

$$\langle g, h \rangle = \int_0^\pi g(x) \overline{h(x)} dx.$$

For $s_k(x) = \sin(kx)$ we have

For $k \neq m$:

$$\int_0^\pi \sin(kx) \sin(mx) dx = 0,$$

For $k = m$:

$$\int_0^\pi \sin^2(kx) dx = \frac{\pi}{2}$$

So s_1, \dots, s_n is an orthogonal set and

$$|s_k|^2 = \langle s_k, s_k \rangle = \frac{\pi}{2}$$

For any constants c_1, \dots, c_n we consider

$$g(x) = \sum_{k=1}^n c_k s_k(x)$$

and since $|f - g|^2 \geq 0$,

$$0 \leq |f - g|^2 = |f|^2 - 2\Re \sum_{k=1}^n c_k \langle f, s_k \rangle + \sum_{k=1}^n |c_k|^2 |s_k|^2$$

using $|s_k|^2 = \pi/2$, this is

$$0 \leq |f|^2 - 2\Re \sum_{k=1}^n c_k \langle f, s_k \rangle + \frac{\pi}{2} \sum_{k=1}^n |c_k|^2 \quad (*)$$

we choose

$$c_k = \frac{2}{\pi} \langle f, s_k \rangle = \frac{2}{\pi} \int_0^\pi f(x) \sin(kx) dx$$

Plug into (*):

Middle term:

$$-2\Re \sum c_k \langle f, s_k \rangle = -2 \sum \frac{2}{\pi} |\langle f, s_k \rangle|^2 = -\frac{4}{\pi} \sum_{k=1}^n |\langle f, s_k \rangle|^2$$

Last term:

$$\frac{\pi}{2} \sum |c_k|^2 = \frac{\pi}{2} \sum \left(\frac{2}{\pi} \right)^2 |\langle f, s_k \rangle|^2 = \frac{2}{\pi} \sum_{k=1}^n |\langle f, s_k \rangle|^2$$

so

$$0 \leq |f|^2 - \frac{4}{\pi} \sum |\langle f, s_k \rangle|^2 + \frac{2}{\pi} \sum |\langle f, s_k \rangle|^2 = |f|^2 - \frac{2}{\pi} \sum_{k=1}^n |\langle f, s_k \rangle|^2$$

rearranging:

$$\sum_{k=1}^n |\langle f, s_k \rangle|^2 \leq \frac{\pi}{2} |f|^2$$

Finally, $\langle f, s_k \rangle = \int_0^\pi f(x) \sin(kx) dx$ and $|f|^2 = \int_0^\pi |f(x)|^2 dx$, so this is exactly

$$\sum_{k=1}^n \left| \int_0^\pi f(x) \sin(kx) dx \right|^2 \leq \frac{\pi}{2} \int_0^\pi |f(x)|^2 dx$$

Question 4

$$\frac{\partial u}{\partial t} = k_1 \frac{\partial^2 u}{\partial x^2} + k_2 \frac{\partial^2 u}{\partial y^2}, \quad 0 < x < L; 0 < y < H,$$

with $u(0, y, t) = u(L, y, t) = 0$ (Dirichlet in (x)),
 $u_y(x, 0, t) = u_y(x, H, t) = 0$ (Neumann in (y)),
and $u(x, y, 0) = \alpha(x, y)$

SoV:

$$\begin{aligned} u(x, y, t) &= X(x)Y(y)T(t) \\ XYT' &= k_1 X''YT + k_2 XY''T \\ \frac{T'}{T} &= k_1 \frac{X''}{X} + k_2 \frac{Y''}{Y} \\ \frac{T'}{T} &= -\lambda, \quad k_1 \frac{X''}{X} + k_2 \frac{Y''}{Y} = -\lambda. \\ k_1 \frac{X''}{X} + k_2 \frac{Y''}{Y} &= -\lambda \Rightarrow \frac{X''}{X} + \frac{k_2}{k_1} \frac{Y''}{Y} = -\frac{\lambda}{k_1}. \end{aligned}$$

separating again with another constant $-\mu$:

$$\frac{X''}{X} = -\mu, \quad \frac{k_2}{k_1} \frac{Y''}{Y} = -\left(\frac{\lambda}{k_1} - \mu\right)$$

ODEs:

$$X'' + \mu X = 0, \quad Y'' + \nu Y = 0, \quad T' + \lambda T = 0,$$

where: $\nu = \frac{k_1}{k_2} \left(\frac{\lambda}{k_1} - \mu \right)$

For x: $X'' + \mu X = 0$, $X(0) = X(L) = 0$

$$\mu_n = \left(\frac{n\pi}{L} \right)^2, \quad X_n(x) = \sin \frac{n\pi x}{L}, \quad n = 1, 2, \dots$$

For y: $Y'' + \nu Y = 0$, $Y'(0) = Y'(H) = 0$

We have a neumann eigenproblem:

$$\nu_m = \left(\frac{m\pi}{H} \right)^2, \quad Y_m(y) = \cos \frac{m\pi y}{H}, \quad m = 0, 1, 2, \dots$$

For each pair $((n, m))$,

$$\lambda_{nm} = k_1 \mu_n + k_2 \nu_m = k_1 \left(\frac{n\pi}{L} \right)^2 + k_2 \left(\frac{m\pi}{H} \right)^2$$

$$T_{nm}(t) = e^{-\lambda_{nm}t}$$

$$u(x, y, t) = \sum_{n=1}^{\infty} \sum_{m=0}^{\infty} A_{nm} \times e^{-(k_1(n\pi/L)^2 + k_2(m\pi/H)^2)t} \sin \frac{n\pi x}{L} \times \cos \frac{m\pi y}{H}$$

At $t = 0$,

$$\alpha(x, y) = u(x, y, 0) = \sum_{n=1}^{\infty} \sum_{m=0}^{\infty} A_{nm} \sin \frac{n\pi x}{L} \cos \frac{m\pi y}{H}$$

so α is expanded in the mixed sin-cos part
using orthogonality:

$$\int_0^L \sin \frac{n\pi x}{L} \sin \frac{p\pi x}{L} dx = \frac{L}{2} \delta_{np}, \quad \int_0^H \cos \frac{m\pi y}{H} \cos \frac{q\pi y}{H} dy = \begin{cases} H, & m = q = 0, \\ \frac{H}{2} \delta_{mq}, & m, q \geq 1. \end{cases}$$

we get

for $m \geq 1$:

$$A_{nm} = \frac{4}{LH} \int_0^L \int_0^H \alpha(x, y) \sin \frac{n\pi x}{L} \cos \frac{m\pi y}{H} dy dx;$$

for $m = 0$:

$$A_{n0} = \frac{2}{LH} \int_0^L \int_0^H \alpha(x, y) \sin \frac{n\pi x}{L} dy dx.$$

$$u(x, y, t) = \sum_{n=1}^{\infty} \sum_{m=0}^{\infty} A_{nm} e^{-\left(k_1 \left(\frac{n\pi}{L}\right)^2 + k_2 \left(\frac{m\pi}{H}\right)^2\right)t} \sin \frac{n\pi x}{L} \cos \frac{m\pi y}{H}$$

with A_{nm} determined from $\alpha(x, y)$ by the formulas above

Question 5

$$c(x, y, z)\rho(x, y, z)\frac{\partial u}{\partial t} = \nabla \cdot (K_0(x, y, z)\nabla u)$$

$$u(x, y, z, t) = \phi(x, y, z)h(t)$$

$$\phi h' = \frac{1}{c\rho}(\nabla \cdot (K_0(h(t)\nabla\phi))) = \frac{h}{c\rho}\nabla \cdot (K_0\nabla\phi)$$

since K_0 depends only on space (last part)

$$\frac{h'}{h} = \frac{1}{c\rho\phi}\nabla \cdot (K_0\nabla\phi)$$

equate to $-\lambda$

$$\frac{h'}{h} = \frac{1}{c\rho\phi}\nabla \cdot (K_0\nabla\phi) = -\lambda$$

$$\frac{h'}{h} = -\lambda \quad \frac{1}{c\rho\phi}\nabla \cdot (K_0\nabla\phi) = -\lambda$$

from the first h :

$$h(t) = Ce^{-\lambda t}$$

$$\nabla \cdot (K_0\nabla\phi) = -\lambda c\rho\phi \iff \nabla \cdot (K_0\nabla\phi) + \lambda c\rho\phi = 0$$

because we have $u = 0$ at the bds for all t and $u = \phi h$, we must have $\phi = 0$ on the region $\partial\Omega$

we just found the eigenvalue eq.:

$$\nabla \cdot (K_0\nabla\phi) + \lambda c\rho\phi = 0$$

and it matches expected

$$\nabla \cdot (p\nabla\phi) + \lambda\sigma(x, y, z)\phi = 0$$

$p(x, y, z) = K_0(x, y, z) \quad \sigma(x, y, z) = c(x, y, z)\rho(x, y, z)$
